substitution/substitution_lemmas.v
@@ -1447,15 +1447,23 @@ revert n d c. induction I; intros; simpl in *. auto.
 destruct n; simpl; auto.
 Qed.
 
-Fixpoint v_shift_inst I v s d cut:
-  f_opt (v_inst v I s) (fun v' => Some (Sub.v_shift v' d cut)) 
-  = v_inst v (inst_shift I d cut) s
-with c_shift_inst I c s d cut:
-  f_opt (c_inst c I s) (fun c' => Some (Sub.c_shift c' d cut)) 
-  = c_inst c (inst_shift I d cut) s
-with h_shift_inst I h s d cut:
-  f_opt (h_inst h I s) (fun h' => Some (Sub.h_shift h' d cut)) 
-  = h_inst h (inst_shift I d cut) s.
+Lemma InstU_shift cut i I d x:
+  i < cut -> 
+  InstU (inst_shift I d cut) (Var (x, i)) 
+  = inst_shift (InstU I (Var (x, i))) d cut.
+Proof.
+intros cmp. simpl. apply leb_correct_conv in cmp. rewrite cmp. auto.
+Qed.
+
+Fixpoint v_shift_inst I v d cut:
+  f_opt (v_inst v I) (fun v' => Some (Sub.v_shift v' d cut)) 
+  = v_inst v (inst_shift I d cut)
+with c_shift_inst I c d cut:
+  f_opt (c_inst c I) (fun c' => Some (Sub.c_shift c' d cut)) 
+  = c_inst c (inst_shift I d cut)
+with h_shift_inst I h d cut:
+  f_opt (h_inst h I) (fun h' => Some (Sub.h_shift h' d cut)) 
+  = h_inst h (inst_shift I d cut).
 Proof.
 all: rename v_shift_inst into VL.
 all: rename c_shift_inst into CL.
@@ -1463,95 +1471,127 @@ all: rename h_shift_inst into HL.
 {
 destruct v; simpl; eauto.
 + destruct v. erewrite <-get_inst_val_shift. auto. 
-+ specialize (VL I v s d cut) as IHv.
++ specialize (VL I v d cut) as IHv.
   clear VL CL HL. rewrite <-IHv.
-  destruct (v_inst v I s); simpl; auto.
-+ specialize (VL I v s d cut) as IHv.
+  destruct (v_inst v I); simpl; auto.
++ specialize (VL I v d cut) as IHv.
   clear VL CL HL. rewrite <-IHv.
-  destruct (v_inst v I s); simpl; auto.
-+ specialize (VL I v1 s d cut) as IHv1.
-  specialize (VL I v2 s d cut) as IHv2.
+  destruct (v_inst v I); simpl; auto.
++ specialize (VL I v1 d cut) as IHv1.
+  specialize (VL I v2 d cut) as IHv2.
   clear VL CL HL. rewrite <-IHv1, <-IHv2.
-  destruct (v_inst v1 I s); simpl; auto.
-  destruct (v_inst v2 I s); simpl; auto.
-+ specialize (VL I v1 s d cut) as IHv1.
-  specialize (VL I v2 s d cut) as IHv2.
+  destruct (v_inst v1 I); simpl; auto.
+  destruct (v_inst v2 I); simpl; auto.
++ specialize (VL I v1 d cut) as IHv1.
+  specialize (VL I v2 d cut) as IHv2.
   clear VL CL HL. rewrite <-IHv1, <-IHv2.
-  destruct (v_inst v1 I s); simpl; auto.
-  destruct (v_inst v2 I s); simpl; auto.
-+ specialize (CL (inst_shift I 1 0) c (S s) d (1+cut)) as IHc.
-  clear VL CL HL. rewrite inst_shift_comm, <-IHc. simpl. 2: omega.
-  destruct (c_inst c (inst_shift I 1 0) (S s)); simpl; auto.
-+ specialize (CL (inst_shift I 1 0) c (S s) d (1+cut)) as IHc.
-  specialize (HL I h s d cut) as IHh.
-  clear VL CL HL. rewrite inst_shift_comm, <-IHc, <-IHh. simpl. 2: omega.
-  destruct (c_inst c (inst_shift I 1 0) (S s)); simpl; auto.
-  destruct (h_inst h I s); simpl; auto.
+  destruct (v_inst v1 I); simpl; auto.
+  destruct (v_inst v2 I); simpl; auto.
++ remember (InstU (inst_shift I 1 0) (Var (v, 0))) as I'.
+  specialize (CL I' c d (1+cut)) as IHc.
+  clear VL CL HL. 
+  rewrite inst_shift_comm, (InstU_shift (1+cut)), <-HeqI', <-IHc.
+  destruct (c_inst c I'); simpl; auto.
+  all: omega.
++ remember (InstU (inst_shift I 1 0) (Var (v, 0))) as I'.
+  specialize (CL I' c d (1+cut)) as IHc.
+  specialize (HL I h d cut) as IHh.
+  clear VL CL HL. 
+  rewrite inst_shift_comm, (InstU_shift (1+cut)), <-HeqI', <-IHc, <-IHh.
+  destruct (c_inst c I'); simpl; auto.
+  destruct (h_inst h I); simpl; auto.
+  all: omega.
 }{
 destruct c; simpl; eauto.
-+ specialize (VL I v s d cut) as IHv.
++ specialize (VL I v d cut) as IHv.
   clear VL CL HL. rewrite <-IHv. simpl.
-  destruct (v_inst v I s); simpl; auto.
-+ specialize (VL I v s d cut) as IHv.
+  destruct (v_inst v I ); simpl; auto.
++ specialize (VL I v d cut) as IHv.
   clear VL CL HL. rewrite <-IHv. simpl.
-  destruct (v_inst v I s); simpl; auto.
-+ specialize (VL I v s d cut) as IHv.
-  specialize (CL (inst_shift I 2 0) c (S(S s)) d (2+cut)) as IHc.
-  clear VL CL HL. rewrite inst_shift_comm, <-IHc, <-IHv. simpl. 2: omega.
-  destruct (v_inst v I s); simpl; auto.
-  destruct (c_inst c (inst_shift I 2 0) (S(S s))); simpl; auto.
-+ specialize (VL I v s d cut) as IHv.
-  specialize (CL (inst_shift I 1 0) c1 (S s) d (1+cut)) as IHc1.
-  specialize (CL (inst_shift I 1 0) c2 (S s) d (1+cut)) as IHc2.
-  clear VL CL HL. rewrite <-IHv. simpl.
-  destruct (v_inst v I s); simpl; auto.
-  rewrite inst_shift_comm, <-IHc1, <-IHc2. simpl. 2: omega.
-  destruct (c_inst c1 (inst_shift I 1 0) (S s)); simpl; auto.
-  destruct (c_inst c2 (inst_shift I 1 0) (S s)); simpl; auto.
-+ specialize (VL I v s d cut) as IHv.
-  specialize (CL I c1 s d cut) as IHc1.
-  specialize (CL (inst_shift I 2 0) c2 (S(S s)) d (2+cut)) as IHc2.
-  clear VL CL HL. rewrite <-IHv. simpl.
-  destruct (v_inst v I s); simpl; auto.
-  rewrite inst_shift_comm, <-IHc1, <-IHc2. simpl. 2: omega.
-  destruct (c_inst c1 I s); simpl; auto.
-  destruct (c_inst c2 (inst_shift I 2 0) (S(S s))); simpl; auto.
-+ specialize (VL I v s d cut) as IHv1.
-  specialize (VL I v0 s d cut) as IHv2.
-  clear VL CL HL. rewrite <-IHv1, <-IHv2.
-  destruct (v_inst v I s); simpl; auto.
-  destruct (v_inst v0 I s); simpl; auto.
-+ specialize (VL I v s d cut) as IHv.
-  specialize (CL (inst_shift I 1 0) c (S s) d (1+cut)) as IHc.
-  clear VL CL HL. rewrite inst_shift_comm, <-IHc, <-IHv. simpl. 2: omega.
-  destruct (v_inst v I s); simpl; auto.
-  destruct (c_inst c (inst_shift I 1 0) (S s)); simpl; auto.
-+ specialize (CL (inst_shift I 2 0) c1 (S(S s)) d (2+cut)) as IHc1.
-  specialize (CL (inst_shift I 1 0) c2 (S s) d (1+cut)) as IHc2.
-  clear VL CL HL.
-  rewrite inst_shift_comm, <-IHc1, inst_shift_comm, <-IHc2. simpl.
-  destruct (c_inst c1 (inst_shift I 2 0) (S(S s))); simpl; auto.
-  destruct (c_inst c2 (inst_shift I 1 0) (S s)); simpl; auto.
-  omega. omega.
-+ specialize (CL I c1 s d cut) as IHc1.
-  specialize (CL (inst_shift I 1 0) c2 (S s) d (1+cut)) as IHc2.
+  destruct (v_inst v I ); simpl; auto.
++ remember (InstU (InstU (inst_shift I 2 0) (Var (v0, 1))) (Var (v1, 0))) as I'.
+  specialize (VL I v d cut) as IHv.
+  specialize (CL I' c d (2+cut)) as IHc.
   clear VL CL HL. 
-  rewrite inst_shift_comm, <-IHc1, <-IHc2. simpl. 2: omega.
-  destruct (c_inst c1 I s); simpl; auto.
-  destruct (c_inst c2 (inst_shift I 1 0) (S s)); simpl; auto.
-+ specialize (VL I v s d cut) as IHv.
-  specialize (CL I c s d cut) as IHc.
+  rewrite inst_shift_comm, (InstU_shift (2+cut)), (InstU_shift (2+cut)). 
+  rewrite <-HeqI', <-IHc, <-IHv. simpl.
+  destruct (v_inst v I ); simpl; auto.
+  destruct (c_inst c I'); simpl; auto.
+  all: omega.
++ remember (InstU (inst_shift I 1 0) (Var (v0, 0))) as I'.
+  remember (InstU (inst_shift I 1 0) (Var (v1, 0))) as I''.
+  specialize (VL I v d cut) as IHv.
+  specialize (CL I' c1 d (1+cut)) as IHc1.
+  specialize (CL I'' c2 d (1+cut)) as IHc2.
+  clear VL CL HL. rewrite <-IHv. simpl.
+  destruct (v_inst v I); simpl; auto.
+  rewrite inst_shift_comm, (InstU_shift (1+cut)), (InstU_shift (1+cut)). 
+  rewrite <-HeqI', <-HeqI'', <-IHc1, <-IHc2. simpl. 2: omega.
+  destruct (c_inst c1 I'); simpl; auto.
+  destruct (c_inst c2 I''); simpl; auto.
+  all: omega.
++ remember (InstU (InstU (inst_shift I 2 0) (Var (v0, 1))) (Var (v1, 0))) as I'.
+  specialize (VL I v d cut) as IHv.
+  specialize (CL I c1 d cut) as IHc1.
+  specialize (CL I' c2 d (2+cut)) as IHc2.
+  clear VL CL HL. rewrite <-IHv. simpl.
+  destruct (v_inst v I ); simpl; auto.
+  rewrite inst_shift_comm, (InstU_shift (2+cut)), (InstU_shift (2+cut)).
+  rewrite <-HeqI', <-IHc1, <-IHc2. simpl.
+  destruct (c_inst c1 I); simpl; auto.
+  destruct (c_inst c2 I'); simpl; auto.
+  all: omega.
++ specialize (VL I v d cut) as IHv1.
+  specialize (VL I v0 d cut) as IHv2.
+  clear VL CL HL. rewrite <-IHv1, <-IHv2.
+  destruct (v_inst v I ); simpl; auto.
+  destruct (v_inst v0 I ); simpl; auto.
++ remember (InstU (inst_shift I 1 0) (Var (v0, 0))) as I'.
+  specialize (VL I v d cut) as IHv.
+  specialize (CL I' c d (1+cut)) as IHc.
+  clear VL CL HL. 
+  rewrite inst_shift_comm, (InstU_shift (1+cut)).
+  rewrite <-HeqI', <-IHc, <-IHv. simpl.
+  destruct (v_inst v I ); simpl; auto.
+  destruct (c_inst c I'); simpl; auto.
+  all: omega.
++ remember (InstU (InstU (inst_shift I 2 0) (Var (v0, 1))) (Var (v, 0))) as I'.
+  remember (InstU (inst_shift I 1 0) (Var (v, 0))) as I''.
+  specialize (CL I' c1 d (2+cut)) as IHc1.
+  specialize (CL I'' c2 d (1+cut)) as IHc2.
+  clear VL CL HL.
+  rewrite inst_shift_comm, (InstU_shift (2+cut)), (InstU_shift (2+cut)).
+  rewrite inst_shift_comm, (InstU_shift (1+cut)).
+  rewrite <-HeqI', <-HeqI'', <-IHc1, <-IHc2. simpl.
+  destruct (c_inst c1 I'); simpl; auto.
+  destruct (c_inst c2 I''); simpl; auto.
+  all: omega.
++ remember (InstU (inst_shift I 1 0) (Var (v, 0))) as I'.
+  specialize (CL I c1 d cut) as IHc1.
+  specialize (CL I' c2 d (1+cut)) as IHc2.
+  clear VL CL HL. 
+  rewrite inst_shift_comm, (InstU_shift (1+cut)). 
+  rewrite <-HeqI', <-IHc1, <-IHc2. simpl.
+  destruct (c_inst c1 I ); simpl; auto.
+  destruct (c_inst c2 I'); simpl; auto.
+  all: omega.
++ specialize (VL I v d cut) as IHv.
+  specialize (CL I c d cut) as IHc.
   clear VL CL HL. rewrite <-IHv, <-IHc.
-  destruct (v_inst v I s); simpl; auto.
-  destruct (c_inst c I s); simpl; auto.
+  destruct (v_inst v I); simpl; auto.
+  destruct (c_inst c I); simpl; auto.
 }{
 destruct h; simpl; eauto.
-specialize (HL I h s d cut) as IHh.
-specialize (CL (inst_shift I 2 0) c (S(S s)) d (2+cut)) as IHc.
-clear VL CL HL. rewrite <-IHh. simpl.
-destruct (h_inst h I s); simpl; auto.
-rewrite inst_shift_comm, <-IHc. simpl. 2: omega.
-destruct (c_inst c (inst_shift I 2 0) (S(S s))); simpl; auto.
+remember (InstU (InstU (inst_shift I 2 0) (Var (v, 1))) (Var (v0, 0))) as I'.
+specialize (HL I h d cut) as IHh.
+specialize (CL I' c d (2+cut)) as IHc.
+clear VL CL HL. 
+rewrite <-IHh. simpl.
+destruct (h_inst h I); simpl; auto.
+rewrite inst_shift_comm, (InstU_shift (2+cut)), (InstU_shift (2+cut)).
+rewrite <-HeqI', <-IHc. simpl.
+destruct (c_inst c I'); simpl; auto.
+all: omega.
 }
 Qed.
 
@@ -1564,18 +1604,26 @@ revert n d c. induction I; intros; simpl in *. auto.
 destruct n; simpl; auto.
 Qed.
 
-Fixpoint v_negshift_inst I v s cut:
+Lemma InstU_negshift cut i I d x:
+  i < cut -> 
+  InstU (inst_negshift I d cut) (Var (x, i)) 
+  = inst_negshift (InstU I (Var (x, i))) d cut.
+Proof.
+intros cmp. simpl. apply leb_correct_conv in cmp. rewrite cmp. auto.
+Qed.
+
+Fixpoint v_negshift_inst I v cut:
   inst_no_var I cut ->
-  f_opt (v_inst v I s) (fun v' => Some (Sub.v_negshift v' 1 cut)) 
-  = v_inst v (inst_negshift I 1 cut) s
-with c_negshift_inst I c s cut:
+  f_opt (v_inst v I) (fun v' => Some (Sub.v_negshift v' 1 cut)) 
+  = v_inst v (inst_negshift I 1 cut)
+with c_negshift_inst I c cut:
   inst_no_var I cut ->
-  f_opt (c_inst c I s) (fun c' => Some (Sub.c_negshift c' 1 cut)) 
-  = c_inst c (inst_negshift I 1 cut) s
-with h_negshift_inst I h s cut:
+  f_opt (c_inst c I) (fun c' => Some (Sub.c_negshift c' 1 cut)) 
+  = c_inst c (inst_negshift I 1 cut)
+with h_negshift_inst I h cut:
   inst_no_var I cut ->
-  f_opt (h_inst h I s) (fun h' => Some (Sub.h_negshift h' 1 cut)) 
-  = h_inst h (inst_negshift I 1 cut) s.
+  f_opt (h_inst h I) (fun h' => Some (Sub.h_negshift h' 1 cut)) 
+  = h_inst h (inst_negshift I 1 cut).
 Proof.
 all: rename v_negshift_inst into VL.
 all: rename c_negshift_inst into CL.
@@ -1583,104 +1631,147 @@ all: rename h_negshift_inst into HL.
 {
 intro novar. destruct v; simpl; eauto.
 + destruct v. erewrite <-get_inst_val_negshift. auto. 
-+ specialize (VL I v s cut) as IHv.
++ specialize (VL I v cut) as IHv.
   clear VL CL HL. rewrite <-IHv; auto.
-  destruct (v_inst v I s); simpl; auto.
-+ specialize (VL I v s cut) as IHv.
+  destruct (v_inst v I); simpl; auto.
++ specialize (VL I v cut) as IHv.
   clear VL CL HL. rewrite <-IHv; auto.
-  destruct (v_inst v I s); simpl; auto.
-+ specialize (VL I v1 s cut) as IHv1.
-  specialize (VL I v2 s cut) as IHv2.
+  destruct (v_inst v I); simpl; auto.
++ specialize (VL I v1 cut) as IHv1.
+  specialize (VL I v2 cut) as IHv2.
   clear VL CL HL. rewrite <-IHv1, <-IHv2; auto.
-  destruct (v_inst v1 I s); simpl; auto.
-  destruct (v_inst v2 I s); simpl; auto.
-+ specialize (VL I v1 s cut) as IHv1.
-  specialize (VL I v2 s cut) as IHv2.
+  destruct (v_inst v1 I); simpl; auto.
+  destruct (v_inst v2 I); simpl; auto.
++ specialize (VL I v1 cut) as IHv1.
+  specialize (VL I v2 cut) as IHv2.
   clear VL CL HL. rewrite <-IHv1, <-IHv2; auto.
-  destruct (v_inst v1 I s); simpl; auto.
-  destruct (v_inst v2 I s); simpl; auto.
-+ specialize (CL (inst_shift I 1 0) c (S s) (1+cut)) as IHc.
-  clear VL CL HL. rewrite inst_shift_negshift_comm, <-IHc. simpl.
-  destruct (c_inst c (inst_shift I 1 0) (S s)); simpl; auto.
-  apply inst_no_var_shift. all: omega || assumption.
-+ specialize (CL (inst_shift I 1 0) c (S s) (1+cut)) as IHc.
-  specialize (HL I h s cut) as IHh.
-  clear VL CL HL. rewrite inst_shift_negshift_comm, <-IHc, <-IHh. simpl.
-  destruct (c_inst c (inst_shift I 1 0) (S s)); simpl; auto.
-  destruct (h_inst h I s); simpl; auto.
+  destruct (v_inst v1 I); simpl; auto.
+  destruct (v_inst v2 I); simpl; auto.
++ remember (InstU (inst_shift I 1 0) (Var (v, 0))) as I'.
+  specialize (CL I' c (1+cut)) as IHc.
+  clear VL CL HL. 
+  rewrite inst_shift_negshift_comm, (InstU_negshift (1+cut)), <-HeqI', <-IHc.
+  destruct (c_inst c I'); simpl; auto.
+  subst. simpl. constructor. 
+  2: apply inst_no_var_shift. all: omega || assumption.
++ remember (InstU (inst_shift I 1 0) (Var (v, 0))) as I'.
+  specialize (CL I' c (1+cut)) as IHc.
+  specialize (HL I h cut) as IHh.
+  clear VL CL HL. 
+  rewrite inst_shift_negshift_comm, (InstU_negshift (1+cut)).
+  rewrite <-HeqI', <-IHc, <-IHh.
+  destruct (c_inst c I'); simpl; auto.
+  destruct (h_inst h I); simpl; auto.
+  auto. subst. simpl. constructor.
   2: apply inst_no_var_shift. all: omega || assumption.
 }{
 intro novar. destruct c; simpl; eauto.
-+ specialize (VL I v s cut) as IHv.
-  clear VL CL HL. rewrite <-IHv; auto. simpl.
-  destruct (v_inst v I s); simpl; auto. 
-+ specialize (VL I v s cut) as IHv.
-  clear VL CL HL. rewrite <-IHv; auto. simpl.
-  destruct (v_inst v I s); simpl; auto.
-+ specialize (VL I v s cut) as IHv.
-  specialize (CL (inst_shift I 2 0) c (S(S s)) (2+cut)) as IHc.
-  clear VL CL HL. rewrite inst_shift_negshift_comm, <-IHc, <-IHv. simpl.
-  destruct (v_inst v I s); simpl; auto.
-  destruct (c_inst c (inst_shift I 2 0) (S(S s))); simpl; auto.
-  2: apply inst_no_var_shift. all: omega || assumption.
-+ specialize (VL I v s cut) as IHv.
-  specialize (CL (inst_shift I 1 0) c1 (S s) (1+cut)) as IHc1.
-  specialize (CL (inst_shift I 1 0) c2 (S s) (1+cut)) as IHc2.
++ specialize (VL I v cut) as IHv.
   clear VL CL HL. rewrite <-IHv. simpl.
-  destruct (v_inst v I s); simpl; auto.
-  rewrite inst_shift_negshift_comm, <-IHc1, <-IHc2. simpl.
-  destruct (c_inst c1 (inst_shift I 1 0) (S s)); simpl; auto.
-  destruct (c_inst c2 (inst_shift I 1 0) (S s)); simpl; auto.
-  apply inst_no_var_shift. 3: apply inst_no_var_shift. all: omega || assumption.
-+ specialize (VL I v s cut) as IHv.
-  specialize (CL I c1 s cut) as IHc1.
-  specialize (CL (inst_shift I 2 0) c2 (S(S s)) (2+cut)) as IHc2.
+  destruct (v_inst v I ); simpl; auto.
+  all: omega || assumption.
++ specialize (VL I v cut) as IHv.
   clear VL CL HL. rewrite <-IHv. simpl.
-  destruct (v_inst v I s); simpl; auto.
-  rewrite inst_shift_negshift_comm, <-IHc1, <-IHc2. simpl.
-  destruct (c_inst c1 I s); simpl; auto.
-  destruct (c_inst c2 (inst_shift I 2 0) (S(S s))); simpl; auto.
-  apply inst_no_var_shift. all: omega || assumption.
-+ specialize (VL I v s cut) as IHv1.
-  specialize (VL I v0 s cut) as IHv2.
-  clear VL CL HL. rewrite <-IHv1, <-IHv2; auto.
-  destruct (v_inst v I s); simpl; auto.
-  destruct (v_inst v0 I s); simpl; auto.
-+ specialize (VL I v s cut) as IHv.
-  specialize (CL (inst_shift I 1 0) c (S s) (1+cut)) as IHc.
-  clear VL CL HL. rewrite inst_shift_negshift_comm, <-IHc, <-IHv. simpl.
-  destruct (v_inst v I s); simpl; auto.
-  destruct (c_inst c (inst_shift I 1 0) (S s)); simpl; auto.
-  2: apply inst_no_var_shift. all: omega || assumption.
-+ specialize (CL (inst_shift I 2 0) c1 (S(S s)) (2+cut)) as IHc1.
-  specialize (CL (inst_shift I 1 0) c2 (S s) (1+cut)) as IHc2.
+  destruct (v_inst v I ); simpl; auto.
+  all: omega || assumption.
++ remember (InstU (InstU (inst_shift I 2 0) (Var (v0, 1))) (Var (v1, 0))) as I'.
+  specialize (VL I v cut) as IHv.
+  specialize (CL I' c (2+cut)) as IHc.
   clear VL CL HL. 
-  rewrite inst_shift_negshift_comm, <-IHc1. 
-  rewrite inst_shift_negshift_comm, <-IHc2. simpl.
-  destruct (c_inst c1 (inst_shift I 2 0) (S(S s))); simpl; auto.
-  destruct (c_inst c2 (inst_shift I 1 0) (S s)); simpl; auto.
-  apply inst_no_var_shift. 5: apply inst_no_var_shift. all: omega || assumption.
-+ specialize (CL I c1 s cut) as IHc1.
-  specialize (CL (inst_shift I 1 0) c2 (S s) (1+cut)) as IHc2.
+  rewrite inst_shift_negshift_comm.
+  rewrite (InstU_negshift (2+cut)), (InstU_negshift (2+cut)). 
+  rewrite <-HeqI', <-IHc, <-IHv. simpl.
+  destruct (v_inst v I ); simpl; auto.
+  destruct (c_inst c I'); simpl; auto.
+  auto. subst. constructor. 2: constructor.
+  3: apply inst_no_var_shift. all: simpl; omega || assumption.
++ remember (InstU (inst_shift I 1 0) (Var (v0, 0))) as I'.
+  remember (InstU (inst_shift I 1 0) (Var (v1, 0))) as I''.
+  specialize (VL I v cut) as IHv.
+  specialize (CL I' c1 (1+cut)) as IHc1.
+  specialize (CL I'' c2 (1+cut)) as IHc2.
+  clear VL CL HL. rewrite <-IHv. simpl.
+  destruct (v_inst v I); simpl; auto.
+  rewrite inst_shift_negshift_comm.
+  rewrite (InstU_negshift (1+cut)), (InstU_negshift (1+cut)). 
+  rewrite <-HeqI', <-HeqI'', <-IHc1, <-IHc2. simpl.
+  destruct (c_inst c1 I'); simpl; auto.
+  destruct (c_inst c2 I''); simpl; auto.
+  all: subst; simpl; omega || auto.
+  all: constructor; omega || apply inst_no_var_shift; auto; omega.
++ remember (InstU (InstU (inst_shift I 2 0) (Var (v0, 1))) (Var (v1, 0))) as I'.
+  specialize (VL I v cut) as IHv.
+  specialize (CL I c1 cut) as IHc1.
+  specialize (CL I' c2 (2+cut)) as IHc2.
+  clear VL CL HL. rewrite <-IHv. simpl.
+  destruct (v_inst v I ); simpl; auto.
+  rewrite inst_shift_negshift_comm.
+  rewrite (InstU_negshift (2+cut)), (InstU_negshift (2+cut)).
+  rewrite <-HeqI', <-IHc1, <-IHc2. simpl.
+  destruct (c_inst c1 I); simpl; auto.
+  destruct (c_inst c2 I'); simpl; auto.
+  subst. constructor. 2: constructor.
+  3: apply inst_no_var_shift. all: simpl; omega || assumption.
++ specialize (VL I v cut) as IHv1.
+  specialize (VL I v0 cut) as IHv2.
+  clear VL CL HL. rewrite <-IHv1, <-IHv2.
+  destruct (v_inst v I ); simpl; auto.
+  destruct (v_inst v0 I ); simpl; auto.
+  all: omega || assumption.
++ remember (InstU (inst_shift I 1 0) (Var (v0, 0))) as I'.
+  specialize (VL I v cut) as IHv.
+  specialize (CL I' c (1+cut)) as IHc.
   clear VL CL HL. 
-  rewrite inst_shift_negshift_comm, <-IHc1, <-IHc2. simpl.
-  destruct (c_inst c1 I s); simpl; auto.
-  destruct (c_inst c2 (inst_shift I 1 0) (S s)); simpl; auto.
-  apply inst_no_var_shift. all: omega || assumption.
-+ specialize (VL I v s cut) as IHv.
-  specialize (CL I c s cut) as IHc.
-  clear VL CL HL. rewrite <-IHv, <-IHc; auto.
-  destruct (v_inst v I s); simpl; auto.
-  destruct (c_inst c I s); simpl; auto.
+  rewrite inst_shift_negshift_comm, (InstU_negshift (1+cut)).
+  rewrite <-HeqI', <-IHc, <-IHv. simpl.
+  destruct (v_inst v I ); simpl; auto.
+  destruct (c_inst c I'); simpl; auto.
+  2: subst; constructor; simpl.
+  3: apply inst_no_var_shift. all: simpl; omega || assumption.
++ remember (InstU (InstU (inst_shift I 2 0) (Var (v0, 1))) (Var (v, 0))) as I'.
+  remember (InstU (inst_shift I 1 0) (Var (v, 0))) as I''.
+  specialize (CL I' c1 (2+cut)) as IHc1.
+  specialize (CL I'' c2 (1+cut)) as IHc2.
+  clear VL CL HL.
+  rewrite inst_shift_negshift_comm.
+  rewrite (InstU_negshift (2+cut)), (InstU_negshift (2+cut)).
+  rewrite inst_shift_negshift_comm, (InstU_negshift (1+cut)).
+  rewrite <-HeqI', <-HeqI'', <-IHc1, <-IHc2. simpl.
+  destruct (c_inst c1 I'); simpl; auto.
+  destruct (c_inst c2 I''); simpl; auto.
+  all: subst; omega || auto.
+  all: constructor. 4: constructor.
+  all: (simpl; omega) || apply inst_no_var_shift; auto; omega.
++ remember (InstU (inst_shift I 1 0) (Var (v, 0))) as I'.
+  specialize (CL I c1 cut) as IHc1.
+  specialize (CL I' c2 (1+cut)) as IHc2.
+  clear VL CL HL. 
+  rewrite inst_shift_negshift_comm, (InstU_negshift (1+cut)). 
+  rewrite <-HeqI', <-IHc1, <-IHc2. simpl.
+  destruct (c_inst c1 I ); simpl; auto.
+  destruct (c_inst c2 I'); simpl; auto.
+  subst. constructor.
+  2: apply inst_no_var_shift. all: simpl; omega || assumption.
++ specialize (VL I v cut) as IHv.
+  specialize (CL I c cut) as IHc.
+  clear VL CL HL. rewrite <-IHv, <-IHc.
+  destruct (v_inst v I); simpl; auto.
+  destruct (c_inst c I); simpl; auto.
+  all: omega || assumption.
 }{
 intro novar. destruct h; simpl; eauto.
-specialize (HL I h s cut) as IHh.
-specialize (CL (inst_shift I 2 0) c (S(S s)) (2+cut)) as IHc.
-clear VL CL HL. rewrite <-IHh. simpl.
-destruct (h_inst h I s); simpl; auto.
-rewrite inst_shift_negshift_comm, <-IHc. simpl.
-destruct (c_inst c (inst_shift I 2 0) (S(S s))); simpl; auto.
-apply inst_no_var_shift. all: omega || assumption.
+remember (InstU (InstU (inst_shift I 2 0) (Var (v, 1))) (Var (v0, 0))) as I'.
+specialize (HL I h cut) as IHh.
+specialize (CL I' c (2+cut)) as IHc.
+clear VL CL HL. 
+rewrite <-IHh. simpl.
+destruct (h_inst h I); simpl; auto.
+rewrite inst_shift_negshift_comm.
+rewrite (InstU_negshift (2+cut)), (InstU_negshift (2+cut)).
+rewrite <-HeqI', <-IHc. simpl.
+destruct (c_inst c I'); simpl; auto.
+subst. constructor. 2:constructor.
+3: apply inst_no_var_shift. all: simpl; (omega || assumption).
 }
 Qed.
 
@@ -1693,111 +1784,152 @@ revert n. induction I; intros; simpl in *. auto.
 destruct n; simpl; auto.
 Qed.
 
-Fixpoint v_sub_inst I v s i vs:
-  f_opt (v_inst v I s) (fun v' => Some (Sub.v_sub v' (i, vs))) 
-  = v_inst v (inst_sub I (i, vs)) s
-with c_sub_inst I c s i vs:
-  f_opt (c_inst c I s) (fun c' => Some (Sub.c_sub c' (i, vs))) 
-  = c_inst c (inst_sub I (i, vs)) s
-with h_sub_inst I h s i vs:
-  f_opt (h_inst h I s) (fun h' => Some (Sub.h_sub h' (i, vs))) 
-  = h_inst h (inst_sub I (i, vs)) s.
+Lemma InstU_sub j i vs I x:
+  i < j -> 
+  InstU (inst_sub I (j, vs)) (Var (x, i)) 
+  = inst_sub (InstU I (Var (x, i))) (j, vs).
+Proof.
+intros cmp. simpl. assert (i=?j=false). apply Nat.eqb_neq. omega.
+rewrite H. auto.
+Qed.
+
+Fixpoint v_sub_inst I v i vs:
+  f_opt (v_inst v I) (fun v' => Some (Sub.v_sub v' (i, vs))) 
+  = v_inst v (inst_sub I (i, vs))
+with c_sub_inst I c i vs:
+  f_opt (c_inst c I) (fun c' => Some (Sub.c_sub c' (i, vs))) 
+  = c_inst c (inst_sub I (i, vs))
+with h_sub_inst I h i vs:
+  f_opt (h_inst h I) (fun h' => Some (Sub.h_sub h' (i, vs))) 
+  = h_inst h (inst_sub I (i, vs)).
 Proof.
 all: rename v_sub_inst into VL.
 all: rename c_sub_inst into CL.
 all: rename h_sub_inst into HL.
 {
 destruct v; simpl; eauto.
-+ destruct v. erewrite <-(get_inst_val_sub). auto. 
-+ specialize (VL I v s i vs) as IHv.
-  clear VL CL HL. rewrite <-IHv; auto.
-  destruct (v_inst v I s); simpl; auto.
-+ specialize (VL I v s i vs) as IHv.
-  clear VL CL HL. rewrite <-IHv; auto.
-  destruct (v_inst v I s); simpl; auto.
-+ specialize (VL I v1 s i vs) as IHv1.
-  specialize (VL I v2 s i vs) as IHv2.
-  clear VL CL HL. rewrite <-IHv1, <-IHv2; auto.
-  destruct (v_inst v1 I s); simpl; auto.
-  destruct (v_inst v2 I s); simpl; auto.
-+ specialize (VL I v1 s i vs) as IHv1.
-  specialize (VL I v2 s i vs) as IHv2.
-  clear VL CL HL. rewrite <-IHv1, <-IHv2; auto.
-  destruct (v_inst v1 I s); simpl; auto.
-  destruct (v_inst v2 I s); simpl; auto.
-+ specialize (CL (inst_shift I 1 0) c (S s) (1+i) (Sub.v_shift vs 1 0)) as IHc.
-  clear VL CL HL. rewrite inst_shift_sub, <-IHc. simpl.
-  destruct (c_inst c (inst_shift I 1 0) (S s)); simpl; auto. omega.
-+ specialize (CL (inst_shift I 1 0) c (S s) (1+i) (Sub.v_shift vs 1 0)) as IHc.
-  specialize (HL I h s i vs) as IHh.
-  clear VL CL HL. rewrite inst_shift_sub, <-IHc, <-IHh. simpl.
-  destruct (c_inst c (inst_shift I 1 0) (S s)); simpl; auto.
-  destruct (h_inst h I s); simpl; auto. omega.
++ destruct v. erewrite <-get_inst_val_sub. auto. 
++ specialize (VL I v i vs) as IHv.
+  clear VL CL HL. rewrite <-IHv.
+  destruct (v_inst v I); simpl; auto.
++ specialize (VL I v i vs) as IHv.
+  clear VL CL HL. rewrite <-IHv.
+  destruct (v_inst v I); simpl; auto.
++ specialize (VL I v1 i vs) as IHv1.
+  specialize (VL I v2 i vs) as IHv2.
+  clear VL CL HL. rewrite <-IHv1, <-IHv2.
+  destruct (v_inst v1 I); simpl; auto.
+  destruct (v_inst v2 I); simpl; auto.
++ specialize (VL I v1 i vs) as IHv1.
+  specialize (VL I v2 i vs) as IHv2.
+  clear VL CL HL. rewrite <-IHv1, <-IHv2.
+  destruct (v_inst v1 I); simpl; auto.
+  destruct (v_inst v2 I); simpl; auto.
++ remember (InstU (inst_shift I 1 0) (Var (v, 0))) as I'.
+  specialize (CL I' c (1+i) (Sub.v_shift vs 1 0)) as IHc.
+  clear VL CL HL. 
+  rewrite inst_shift_sub, (InstU_sub (1+i)), <-HeqI', <-IHc.
+  destruct (c_inst c I'); simpl; auto.
+  all: omega.
++ remember (InstU (inst_shift I 1 0) (Var (v, 0))) as I'.
+  specialize (CL I' c (1+i) (Sub.v_shift vs 1 0)) as IHc.
+  specialize (HL I h i vs) as IHh.
+  clear VL CL HL. 
+  rewrite inst_shift_sub, (InstU_sub (1+i)), <-HeqI', <-IHc, <-IHh.
+  destruct (c_inst c I'); simpl; auto.
+  destruct (h_inst h I); simpl; auto.
+  all: omega.
 }{
 destruct c; simpl; eauto.
-+ specialize (VL I v s i vs) as IHv.
-  clear VL CL HL. rewrite <-IHv; auto. simpl.
-  destruct (v_inst v I s); simpl; auto. 
-+ specialize (VL I v s i vs) as IHv.
-  clear VL CL HL. rewrite <-IHv; auto. simpl.
-  destruct (v_inst v I s); simpl; auto.
-+ specialize (VL I v s i vs) as IHv.
-  specialize (CL (inst_shift I 2 0) c (S(S s)) (2+i) (Sub.v_shift vs 2 0)) as IHc.
-  clear VL CL HL. rewrite inst_shift_sub, <-IHc, <-IHv. simpl.
-  destruct (v_inst v I s); simpl; auto.
-  destruct (c_inst c (inst_shift I 2 0) (S(S s))); simpl; auto. omega.
-+ specialize (VL I v s i) as IHv.
-  specialize (CL (inst_shift I 1 0) c1 (S s) (1+i) (Sub.v_shift vs 1 0)) as IHc1.
-  specialize (CL (inst_shift I 1 0) c2 (S s) (1+i) (Sub.v_shift vs 1 0)) as IHc2.
++ specialize (VL I v i vs) as IHv.
   clear VL CL HL. rewrite <-IHv. simpl.
-  destruct (v_inst v I s); simpl; auto.
-  rewrite inst_shift_sub, <-IHc1, <-IHc2. simpl. 2: omega.
-  destruct (c_inst c1 (inst_shift I 1 0) (S s)); simpl; auto.
-  destruct (c_inst c2 (inst_shift I 1 0) (S s)); simpl; auto.
-+ specialize (VL I v s i vs) as IHv.
-  specialize (CL I c1 s i vs) as IHc1.
-  specialize (CL (inst_shift I 2 0) c2 (S(S s)) (2+i) (Sub.v_shift vs 2 0)) as IHc2.
+  destruct (v_inst v I ); simpl; auto.
++ specialize (VL I v i vs) as IHv.
   clear VL CL HL. rewrite <-IHv. simpl.
-  destruct (v_inst v I s); simpl; auto.
-  rewrite inst_shift_sub, <-IHc1, <-IHc2. simpl.
-  destruct (c_inst c1 I s); simpl; auto.
-  destruct (c_inst c2 (inst_shift I 2 0) (S(S s))); simpl; auto. omega.
-+ specialize (VL I v s i) as IHv1.
-  specialize (VL I v0 s i) as IHv2.
-  clear VL CL HL. rewrite <-IHv1, <-IHv2; auto.
-  destruct (v_inst v I s); simpl; auto.
-  destruct (v_inst v0 I s); simpl; auto.
-+ specialize (VL I v s i) as IHv.
-  specialize (CL (inst_shift I 1 0) c (S s) (1+i) (Sub.v_shift vs 1 0)) as IHc.
-  clear VL CL HL. rewrite inst_shift_sub, <-IHc, <-IHv. simpl.
-  destruct (v_inst v I s); simpl; auto.
-  destruct (c_inst c (inst_shift I 1 0) (S s)); simpl; auto. omega.
-+ specialize (CL (inst_shift I 2 0) c1 (S(S s)) (2+i) (Sub.v_shift vs 2 0)) as IHc1.
-  specialize (CL (inst_shift I 1 0) c2 (S s) (1+i) (Sub.v_shift vs 1 0)) as IHc2.
+  destruct (v_inst v I ); simpl; auto.
++ remember (InstU (InstU (inst_shift I 2 0) (Var (v0, 1))) (Var (v1, 0))) as I'.
+  specialize (VL I v i vs) as IHv.
+  specialize (CL I' c (2+i) (Sub.v_shift vs 2 0)) as IHc.
   clear VL CL HL. 
-  rewrite inst_shift_sub, <-IHc1. 
-  rewrite inst_shift_sub, <-IHc2. simpl.
-  destruct (c_inst c1 (inst_shift I 2 0) (S(S s))); simpl; auto.
-  destruct (c_inst c2 (inst_shift I 1 0) (S s)); simpl; auto. omega. omega.
-+ specialize (CL I c1 s i vs) as IHc1.
-  specialize (CL (inst_shift I 1 0) c2 (S s) (1+i) (Sub.v_shift vs 1 0)) as IHc2.
+  rewrite inst_shift_sub, (InstU_sub (2+i)), (InstU_sub (2+i)). 
+  rewrite <-HeqI', <-IHc, <-IHv. simpl.
+  destruct (v_inst v I ); simpl; auto.
+  destruct (c_inst c I'); simpl; auto.
+  all: omega.
++ remember (InstU (inst_shift I 1 0) (Var (v0, 0))) as I'.
+  remember (InstU (inst_shift I 1 0) (Var (v1, 0))) as I''.
+  specialize (VL I v i vs) as IHv.
+  specialize (CL I' c1 (1+i) (Sub.v_shift vs 1 0)) as IHc1.
+  specialize (CL I'' c2 (1+i) (Sub.v_shift vs 1 0)) as IHc2.
+  clear VL CL HL. rewrite <-IHv. simpl.
+  destruct (v_inst v I); simpl; auto.
+  rewrite inst_shift_sub, (InstU_sub (1+i)), (InstU_sub (1+i)). 
+  rewrite <-HeqI', <-HeqI'', <-IHc1, <-IHc2. simpl. 2: omega.
+  destruct (c_inst c1 I'); simpl; auto.
+  destruct (c_inst c2 I''); simpl; auto.
+  all: omega.
++ remember (InstU (InstU (inst_shift I 2 0) (Var (v0, 1))) (Var (v1, 0))) as I'.
+  specialize (VL I v i vs) as IHv.
+  specialize (CL I c1 i vs) as IHc1.
+  specialize (CL I' c2 (2+i) (Sub.v_shift vs 2 0)) as IHc2.
+  clear VL CL HL. rewrite <-IHv. simpl.
+  destruct (v_inst v I ); simpl; auto.
+  rewrite inst_shift_sub, (InstU_sub (2+i)), (InstU_sub (2+i)).
+  rewrite <-HeqI', <-IHc1, <-IHc2. simpl.
+  destruct (c_inst c1 I); simpl; auto.
+  destruct (c_inst c2 I'); simpl; auto.
+  all: omega.
++ specialize (VL I v i vs) as IHv1.
+  specialize (VL I v0 i vs) as IHv2.
+  clear VL CL HL. rewrite <-IHv1, <-IHv2.
+  destruct (v_inst v I ); simpl; auto.
+  destruct (v_inst v0 I ); simpl; auto.
++ remember (InstU (inst_shift I 1 0) (Var (v0, 0))) as I'.
+  specialize (VL I v i vs) as IHv.
+  specialize (CL I' c (1+i) (Sub.v_shift vs 1 0)) as IHc.
   clear VL CL HL. 
-  rewrite inst_shift_sub, <-IHc1, <-IHc2. simpl.
-  destruct (c_inst c1 I s); simpl; auto.
-  destruct (c_inst c2 (inst_shift I 1 0) (S s)); simpl; auto. omega.
-+ specialize (VL I v s i) as IHv.
-  specialize (CL I c s i) as IHc.
-  clear VL CL HL. rewrite <-IHv, <-IHc; auto.
-  destruct (v_inst v I s); simpl; auto.
-  destruct (c_inst c I s); simpl; auto.
+  rewrite inst_shift_sub, (InstU_sub (1+i)).
+  rewrite <-HeqI', <-IHc, <-IHv. simpl.
+  destruct (v_inst v I ); simpl; auto.
+  destruct (c_inst c I'); simpl; auto.
+  all: omega.
++ remember (InstU (InstU (inst_shift I 2 0) (Var (v0, 1))) (Var (v, 0))) as I'.
+  remember (InstU (inst_shift I 1 0) (Var (v, 0))) as I''.
+  specialize (CL I' c1 (2+i) (Sub.v_shift vs 2 0)) as IHc1.
+  specialize (CL I'' c2 (1+i) (Sub.v_shift vs 1 0)) as IHc2.
+  clear VL CL HL.
+  rewrite inst_shift_sub, (InstU_sub (2+i)), (InstU_sub (2+i)).
+  rewrite inst_shift_sub, (InstU_sub (1+i)).
+  rewrite <-HeqI', <-HeqI'', <-IHc1, <-IHc2. simpl.
+  destruct (c_inst c1 I'); simpl; auto.
+  destruct (c_inst c2 I''); simpl; auto.
+  all: omega.
++ remember (InstU (inst_shift I 1 0) (Var (v, 0))) as I'.
+  specialize (CL I c1 i vs) as IHc1.
+  specialize (CL I' c2 (1+i) (Sub.v_shift vs 1 0)) as IHc2.
+  clear VL CL HL. 
+  rewrite inst_shift_sub, (InstU_sub (1+i)). 
+  rewrite <-HeqI', <-IHc1, <-IHc2. simpl.
+  destruct (c_inst c1 I ); simpl; auto.
+  destruct (c_inst c2 I'); simpl; auto.
+  all: omega.
++ specialize (VL I v i vs) as IHv.
+  specialize (CL I c i vs) as IHc.
+  clear VL CL HL. rewrite <-IHv, <-IHc.
+  destruct (v_inst v I); simpl; auto.
+  destruct (c_inst c I); simpl; auto.
 }{
 destruct h; simpl; eauto.
-specialize (HL I h s i) as IHh.
-specialize (CL (inst_shift I 2 0) c (S(S s)) (2+i) (Sub.v_shift vs 2 0)) as IHc.
-clear VL CL HL. rewrite <-IHh. simpl.
-destruct (h_inst h I s); simpl; auto.
-rewrite inst_shift_sub, <-IHc. simpl.
-destruct (c_inst c (inst_shift I 2 0) (S(S s))); simpl; auto. omega.
+remember (InstU (InstU (inst_shift I 2 0) (Var (v, 1))) (Var (v0, 0))) as I'.
+specialize (HL I h i vs) as IHh.
+specialize (CL I' c (2+i) (Sub.v_shift vs 2 0)) as IHc.
+clear VL CL HL. 
+rewrite <-IHh. simpl.
+destruct (h_inst h I); simpl; auto.
+rewrite inst_shift_sub, (InstU_sub (2+i)), (InstU_sub (2+i)).
+rewrite <-HeqI', <-IHc. simpl.
+destruct (c_inst c I'); simpl; auto.
+all: omega.
 }
 Qed.
 
@@ -1810,30 +1942,30 @@ rewrite IHI. f_equal.
 Qed.
 
 
-Fixpoint v_subs_inst I v s vs i:
-  f_opt (v_inst v I s) (fun v' => Some (v_subs v' vs i)) 
-  = v_inst v (inst_subs I vs i) s
-with c_subs_inst I c s vs i:
-  f_opt (c_inst c I s) (fun c' => Some (c_subs c' vs i)) 
-  = c_inst c (inst_subs I vs i) s
-with h_subs_inst I h s vs i:
-  f_opt (h_inst h I s) (fun h' => Some (h_subs h' vs i)) 
-  = h_inst h (inst_subs I vs i) s.
+Fixpoint v_subs_inst I v vs i:
+  f_opt (v_inst v I) (fun v' => Some (v_subs v' vs i)) 
+  = v_inst v (inst_subs I vs i)
+with c_subs_inst I c vs i:
+  f_opt (c_inst c I) (fun c' => Some (c_subs c' vs i)) 
+  = c_inst c (inst_subs I vs i)
+with h_subs_inst I h vs i:
+  f_opt (h_inst h I) (fun h' => Some (h_subs h' vs i)) 
+  = h_inst h (inst_subs I vs i).
 Proof.
 {
 unfold v_subs. rewrite <-inst_subs_unfold.
 rewrite <-v_negshift_inst, <-v_sub_inst.
-destruct (v_inst v I s); simpl; auto.
+destruct (v_inst v I); simpl; auto.
 apply inst_sub_makes_no_var. apply v_shift_makes_no_var.
 }{
 unfold c_subs. rewrite <-inst_subs_unfold.
 rewrite <-c_negshift_inst, <-c_sub_inst.
-destruct (c_inst c I s); simpl; auto.
+destruct (c_inst c I); simpl; auto.
 apply inst_sub_makes_no_var. apply v_shift_makes_no_var.
 }{
 unfold h_subs. rewrite <-inst_subs_unfold.
 rewrite <-h_negshift_inst, <-h_sub_inst.
-destruct (h_inst h I s); simpl; auto.
+destruct (h_inst h I); simpl; auto.
 apply inst_sub_makes_no_var. apply v_shift_makes_no_var.
 }
 Qed.
