type_system/declarational.v
@@ -336,8 +336,8 @@ with ceq' : ctype -> ctx -> comp -> comp -> Prop :=
 | OOTB A Σ E Γ' I Γ Z T1 T2 c1 c2:
     has_eq E Γ Z T1 T2 ->
     wf_inst Γ' I (join_ctxs (tctx_to_ctx Z (CTy A Σ E)) Γ) ->
-    c_inst (tmpl_to_comp (ctx_len Γ) T1) I 0 = Some c1 ->
-    c_inst (tmpl_to_comp (ctx_len Γ) T2) I 0 = Some c2 ->
+    c_inst (tmpl_to_comp (ctx_len Γ) T1) I = Some c1 ->
+    c_inst (tmpl_to_comp (ctx_len Γ) T2) I = Some c2 ->
     ceq' (CTy A Σ E) Γ' c1 c2
 | βΠMatch v1 v2 x y c C Γ: 
     ceq' C Γ
